pulse/lib/pulse/lib/Pulse.Lib.Array.Core.fst
@@ -23,55 +23,14 @@ open PulseCore.FractionalPermission
 open FStar.Ghost
 module SZ = FStar.SizeT
 module Seq = FStar.Seq
-module U = Pulse.Lib.Raise
 
 let base_t = H.base_t
 inline_for_extraction
-let array a = H.array (U.raise_t a)
+let array a = H.array a
 let length #a x = H.length x
 let base_of x = H.base_of x
 let offset_of x = H.offset_of x
 let is_full_array #a x = H.is_full_array x
-let raise_seq (#a:Type0) (x:FStar.Seq.seq a)
-  : FStar.Seq.seq (U.raise_t u#0 u#1 a)
-  = FStar.Seq.map_seq U.raise_val x
-let map_seq_len #a #b (x:FStar.Seq.seq a) (f:a -> b)
-: Lemma (ensures Seq.length (Seq.map_seq f x) ==  Seq.length x)
-        [SMTPat (Seq.length (Seq.map_seq f x))]
-= FStar.Seq.map_seq_len f x
-let map_seq_index #a #b (x:FStar.Seq.seq a) (f:a -> b) (i:nat { i < Seq.length x })
-: Lemma (ensures Seq.index (Seq.map_seq f x) i == f (Seq.index x i))
-        [SMTPat (Seq.index (Seq.map_seq f x) i)]
-= FStar.Seq.map_seq_index f x i
-
-let raise_seq_len #a (x:FStar.Seq.seq a)
-: Lemma (ensures Seq.length (raise_seq x) == Seq.length x)
-        [SMTPat (Seq.length (raise_seq x))]
-= ()//FStar.Seq.map_seq_len (U.raise_val u#0 u#1) x
-let raise_seq_index #a (x:FStar.Seq.seq a) (i:nat)
-: Lemma
-  (requires i < Seq.length x)
-  (ensures Seq.index (raise_seq x) i == U.raise_val u#0 u#1 (Seq.index x i))
-  [SMTPat (Seq.index (raise_seq x) i)]
-=  ()//FStar.Seq.map_seq_index (U.raise_val u#0 u#1) x i
-
-let downgrade_seq #a (x: Seq.seq (U.raise_t u#0 u#1 a)) : Seq.seq a
-= Seq.map_seq U.downgrade_val x
-let raise_seq_downgrade_seq #a (x: Seq.seq (U.raise_t a))
-: Lemma (raise_seq (downgrade_seq x) == x) [SMTPat (raise_seq (downgrade_seq x))]
-= assert Seq.equal (raise_seq (downgrade_seq x)) x
-
-let raise_seq_inv (#elt:Type0) (x:FStar.Seq.seq elt)
-: Lemma (ensures downgrade_seq (raise_seq x)
-                 `Seq.equal` x)
-        [SMTPat (raise_seq x)]
-= ()
-
-let downgrade_seq_inv (#elt:Type0) (x:FStar.Seq.seq (U.raise_t u#0 u#1 elt))
-: Lemma (ensures raise_seq (downgrade_seq x)
-                 `Seq.equal` x)
-        [SMTPat (downgrade_seq x)]
-= ()
 
 inline_for_extraction
 let null #a : array a = H.null
@@ -80,486 +39,73 @@ let is_null r = H.is_null r
 
 [@@pulse_unfold]
 let pts_to_mask #t ([@@@mkey] a: array t) (#[full_default()] f: perm) (v: erased (Seq.seq t)) (mask: nat -> prop) : slprop =
-  H.pts_to_mask a #f (raise_seq v) mask
+  H.pts_to_mask a #f v mask
 
 let pts_to_mask_timeless (#a:Type) (x:array a) (p:perm) (s:Seq.seq a) mask =
   ()
 
-ghost
-fn pts_to_mask_len #t (a:array t) (#p:perm) (#x:Seq.seq t) #mask
-  preserves pts_to_mask a #p x mask
-  ensures pure (length a == Seq.length x)
-{
-  H.pts_to_mask_len a;
-}
+let pts_to_mask_len a = H.pts_to_mask_len a
+let pts_to_mask_not_null r = H.pts_to_mask_not_null r
 
-ghost
-fn pts_to_mask_not_null #a #p (r:array a) (#v:Seq.seq a) #mask
-  preserves pts_to_mask r #p v mask
-  ensures pure (not (is_null r))
-{
-  H.pts_to_mask_not_null r;
-}
+let mask_vext arr = H.mask_vext arr
+let mask_mext arr = H.mask_mext arr
+let mask_ext arr = H.mask_ext arr
 
-ghost fn mask_vext #t (arr: array t) #f #v v' #mask
-  requires pts_to_mask arr #f v mask
-  requires pure (Seq.length v' == Seq.length v /\
-    (forall (i: nat). mask i /\ i < Seq.length v ==> Seq.index v i == Seq.index v' i))
-  ensures pts_to_mask arr #f v' mask
-{
-  H.mask_vext arr (raise_seq v');
-}
+let mask_share arr = H.mask_share arr
+let mask_gather arr = H.mask_gather arr
 
-ghost fn mask_mext #t (arr: array t) #f #v #mask (mask': nat -> prop)
-  requires pts_to_mask arr #f v mask
-  requires pure (forall (i: nat). i < Seq.length v ==> (mask i <==> mask' i))
-  ensures pts_to_mask arr #f v mask'
-{
-  H.mask_mext arr mask';
-}
+let split_mask arr = H.split_mask arr
+let join_mask arr = H.join_mask arr
+let join_mask' arr = H.join_mask' arr
 
-ghost fn mask_ext #t (arr: array t) #f #v #mask v' (mask': nat -> prop)
-  requires pts_to_mask arr #f v mask
-  requires pure (forall (i: nat). i < Seq.length v ==> (mask i <==> mask' i))
-  requires pure (Seq.length v' == Seq.length v /\
-    (forall (i: nat). mask i /\ i < Seq.length v ==> Seq.index v i == Seq.index v' i))
-  ensures pts_to_mask arr #f v' mask'
-{
-  H.mask_ext arr (raise_seq v') mask';
-}
+let pts_to_mask_injective_eq arr = H.pts_to_mask_injective_eq arr
 
-ghost
-fn mask_share #a (arr:array a) (#s: Seq.seq a) #p #mask
-  requires pts_to_mask arr #p s mask
-  ensures pts_to_mask arr #(p /. 2.0R) s mask
-  ensures pts_to_mask arr #(p /. 2.0R) s mask
-{
-  H.mask_share arr;
-}
+inline_for_extraction let mask_read a = H.mask_read a
+inline_for_extraction let mask_write a = H.mask_write a
 
-[@@allow_ambiguous]
-ghost fn mask_gather #t (arr: array t) #p1 #p2 #s1 #s2 #mask1 #mask2
-  requires pts_to_mask arr #p1 s1 mask1
-  requires pts_to_mask arr #p2 s2 mask2
-  requires pure (forall i. mask1 i <==> mask2 i)
-  ensures exists* (v: Seq.seq t). pts_to_mask arr #(p1 +. p2) v mask1 **
-    pure ((Seq.length v == Seq.length s1 /\ Seq.length v == Seq.length s2) /\
-      (forall (i: nat). i < Seq.length v /\ mask1 i ==> Seq.index v i == Seq.index s1 i /\ Seq.index v i == Seq.index s2 i))
-{
-  H.mask_gather arr;
-  H.mask_mext arr mask1;
-  with v. assert H.pts_to_mask arr #(p1 +. p2) v mask1;
-  fold pts_to_mask arr #(p1 +. p2) (downgrade_seq v) mask1;
-}
+let gsub arr = H.gsub arr
 
-ghost fn split_mask #t (arr: array t) #f #v #mask (pred: nat -> prop)
-  requires pts_to_mask arr #f v mask
-  ensures pts_to_mask arr #f v (mask_isect mask pred)
-  ensures pts_to_mask arr #f v (mask_diff mask pred)
-{
-  H.split_mask arr pred;
-}
+let gsub_intro arr = H.gsub_intro arr
+let gsub_elim arr = H.gsub_elim arr
 
-[@@allow_ambiguous]
-ghost fn join_mask #t (arr: array t) #f #v1 #v2 #mask1 #mask2
-  requires pts_to_mask arr #f v1 mask1
-  requires pts_to_mask arr #f v2 mask2
-  requires pure (forall i. ~(mask1 i /\ mask2 i))
-  ensures exists* (v: Seq.seq t).
-    pts_to_mask arr #f v (fun i -> mask1 i \/ mask2 i) **
-    pure (Seq.length v == Seq.length v1 /\ Seq.length v == Seq.length v2 /\
-      (forall (i: nat). i < Seq.length v ==>
-        (mask1 i ==> Seq.index v i == Seq.index v1 i) /\
-        (mask2 i ==> Seq.index v i == Seq.index v2 i)))
-{
-  H.join_mask arr #f #_ #_ #mask1 #mask2;
-  with v. assert H.pts_to_mask arr #f v (fun i -> mask1 i \/ mask2 i);
-  fold pts_to_mask arr #f (downgrade_seq v) (fun i -> mask1 i \/ mask2 i);
-}
+inline_for_extraction let sub arr = H.sub arr
+let return_sub arr = H.return_sub arr
 
-[@@allow_ambiguous]
-ghost fn join_mask' #t (arr: array t) #f (#v: erased (Seq.seq t)) #mask1 #mask2
-  requires pts_to_mask arr #f v mask1
-  requires pts_to_mask arr #f v mask2
-  requires pure (forall i. ~(mask1 i /\ mask2 i))
-  ensures pts_to_mask arr #f v (fun i -> mask1 i \/ mask2 i)
-{
-  H.join_mask' arr #_ #_ #mask1 #mask2;
-}
+let pts_to r = H.pts_to r
 
-[@@allow_ambiguous]
-ghost
-fn pts_to_mask_injective_eq #a #p0 #p1 #s0 #s1 #mask0 #mask1 (arr:array a)
-  preserves pts_to_mask arr #p0 s0 mask0
-  preserves pts_to_mask arr #p1 s1 mask1
-  ensures pure (Seq.length s0 == Seq.length s1 /\
-    (forall (i: nat). i < Seq.length s0 /\ mask0 i /\ mask1 i ==>
-      Seq.index s0 i == Seq.index s1 i))
-{
-  H.pts_to_mask_injective_eq arr;
-}
-
-inline_for_extraction
-fn mask_read #t (a: array t) (i: SZ.t) #p (#s: erased (Seq.seq t) { SZ.v i < Seq.length s }) #mask
-  preserves pts_to_mask a #p s mask
-  requires pure (mask (SZ.v i))
-  returns res: t
-  ensures pure (res == Seq.index s (SZ.v i))
-{
-  U.downgrade_val (H.mask_read a i)
-}
-
-inline_for_extraction
-fn mask_write #t (a: array t) (i: SZ.t) (v: t) (#s: erased (Seq.seq t) { SZ.v i < Seq.length s }) #mask
-  requires pts_to_mask a s mask
-  requires pure (mask (SZ.v i))
-  ensures pts_to_mask a (Seq.upd s (SZ.v i) v) mask
-{
-  H.mask_write a i (U.raise_val v);
-  with s'. assert H.pts_to_mask a s' mask;
-  assert pure (Seq.equal s' (raise_seq (Seq.upd s (SZ.v i) v)));
-}
-
-let gsub #t (arr: array t) (i: nat) (j: nat { i <= j /\ j <= length arr }) : GTot (array t) =
-  H.gsub arr i j
-
-ghost fn gsub_intro #t (arr: array t) #f #mask (i j: nat) (#v: erased (Seq.seq t) { i <= j /\ j <= Seq.length v })
-  requires pts_to_mask arr #f v mask
-  requires pure (forall (k: nat). mask k ==> i <= k /\ k < j)
-  returns _: squash (length arr == Seq.length v)
-  ensures pts_to_mask (gsub arr i j) #f (Seq.slice v i j) (fun k -> mask (k + i))
-{
-  H.gsub_intro arr i j;
-  with v'. assert H.pts_to_mask (gsub arr i j) #f v' (fun k -> mask (k + i));
-  assert pure (Seq.equal v' (raise_seq (Seq.slice v i j)));
-}
-
-ghost fn gsub_elim #t (arr: array t) #f (#mask: nat->prop) (i j: nat)
-    (#v: erased (Seq.seq t) { i <= j /\ j <= length arr })
-  requires pts_to_mask (gsub arr i j) #f v mask
-  returns _: squash (j - i == Seq.length v)
-  ensures exists* v'.
-    pts_to_mask arr #f v' (fun k -> i <= k /\ k < j /\ mask (k - i)) **
-    pure (Seq.length v' == length arr /\ (forall (k:nat). k < j - i ==> Seq.index v k == Seq.index v' (k + i)))
-{
-  H.gsub_elim arr i j;
-  with v' mask'. assert H.pts_to_mask arr #f v' mask';
-  assert pts_to_mask arr #f (downgrade_seq v') mask';
-}
-
-inline_for_extraction
-unobservable
-fn sub #t (arr: array t) #f #mask (i: SZ.t) (j: SZ.t)
-    (#v: erased (Seq.seq t) { SZ.v i <= SZ.v j /\ SZ.v j <= Seq.length (reveal v) })
-  requires pts_to_mask arr #f v mask
-  returns sub: (sub: array t { length arr == Seq.length (reveal v) })
-  ensures rewrites_to sub (gsub arr (SZ.v i) (SZ.v j))
-  ensures pts_to_mask sub #f (Seq.slice v (SZ.v i) (SZ.v j)) (fun k -> mask (k + SZ.v i))
-  ensures pts_to_mask arr #f v (fun k -> mask k /\ ~(SZ.v i <= k /\ k < SZ.v j))
-{
-  let sub = H.sub arr i j #(raise_seq v);
-  with v' mask'. assert H.pts_to_mask sub #f v' mask';
-  assert pure (Seq.equal v' (raise_seq (Seq.slice v (SZ.v i) (SZ.v j))));
-  sub
-}
-
-[@@allow_ambiguous]
-ghost fn return_sub #t (arr: array t) #f (#v #vsub: erased (Seq.seq t)) #mask #masksub (#i: nat) (#j: nat { i <= j /\ j <= length arr })
-  requires pts_to_mask arr #f v mask
-  requires pts_to_mask (gsub arr i j) #f vsub masksub
-  requires pure (forall (k: nat). i <= k /\ k < j ==> ~(mask k))
-  ensures exists* v'. pts_to_mask arr #f v' (fun k -> mask k \/ (i <= k /\ k < j /\ masksub (k - i)))
-    ** pure (Seq.length v == Seq.length v' /\ i + Seq.length vsub == j /\ j <= Seq.length v /\
-      (forall (k: nat). k < Seq.length v' ==>
-      Seq.index v' k == (if i <= k && k < j then Seq.index vsub (k - i) else Seq.index v k)))
-{
-  H.return_sub arr;
-  with v' mask'. assert H.pts_to_mask arr #f v' mask';
-  assert pts_to_mask arr #f (downgrade_seq v') mask';
-}
-
-let pts_to #a 
-    (r:array a)
-    (#[exact (`1.0R)] p:perm)
-    (v:FStar.Seq.seq a)
-= H.pts_to r #p (raise_seq v)
-
-ghost fn to_mask #t (arr: array t) #f #v
-  requires arr |-> Frac f v
-  ensures pts_to_mask arr #f v (fun _ -> True)
-{
-  unfold pts_to arr #f v;
-  H.to_mask arr;
-}
-
-ghost fn from_mask #t (arr: array t) #f #v #mask
-  requires pts_to_mask arr #f v mask
-  requires pure (forall i. mask i)
-  ensures arr |-> Frac f v
-{
-  H.from_mask arr;
-  fold pts_to arr #f v;
-}
+let to_mask arr = H.to_mask arr
+let from_mask arr = H.from_mask arr
 
 let pts_to_timeless _ _ _ = ()
+let pts_to_len a = H.pts_to_len a
 
+inline_for_extraction let alloc x = H.alloc x
 
-ghost
-fn pts_to_len (#t:Type) (a:array t) (#p:perm) (#x:FStar.Seq.seq t)
-  requires pts_to a #p x
-  ensures pts_to a #p x ** pure (length a == Seq.length x)
-{
-  unfold (pts_to a #p x);
-  H.pts_to_len a;
-  fold (pts_to a #p x)
-}
+inline_for_extraction let op_Array_Access a = H.op_Array_Access a
+inline_for_extraction let op_Array_Assignment a = H.op_Array_Assignment a
 
+inline_for_extraction let free a = H.free a
 
+let share arr = H.share arr
+let gather arr = H.gather arr
 
-inline_for_extraction
-fn alloc (#elt:Type0) (x:elt) (n:SZ.t)
-  requires emp
-  returns a:array elt
-ensures
-  pts_to a (Seq.create (SZ.v n) x) **
-  pure (length a == SZ.v n /\ is_full_array a)
-{
-  let a = H.alloc (U.raise_val x) n;
-  with w. assert H.pts_to a w;
-  assert pure (raise_seq (Seq.create (SZ.v n) x) `Seq.equal` w);
-  fold (pts_to a (Seq.create (SZ.v n) x));
-  a
-}
-
-
-
-inline_for_extraction
-fn op_Array_Access
-    (#t: Type)
-    (a: array t)
-    (i: SZ.t)
-    (#p: perm)
-    (#s: Ghost.erased (Seq.seq t){SZ.v i < Seq.length s})
-preserves pts_to a #p s
-returns res:t
-ensures rewrites_to res (Seq.index s (SZ.v i))
-{
-  unfold (pts_to a #p s);
-  let res = H.(a.(i));
-  fold (pts_to a #p s);
-  U.downgrade_val res
-}
-
-
-
-inline_for_extraction
-fn op_Array_Assignment
-    (#t: Type)
-    (a: array t)
-    (i: SZ.t)
-    (v: t)
-    (#s: Ghost.erased (Seq.seq t) {SZ.v i < Seq.length s})
-requires
-  pts_to a s
-ensures
-  pts_to a (Seq.upd s (SZ.v i) v)
-{
-  unfold (pts_to a s);
-  H.(a.(i) <- U.raise_val v);
-  with w. assert H.pts_to a w;
-  assert pure (raise_seq (Seq.upd s (SZ.v i) v) `Seq.equal` w);
-  fold (pts_to a (Seq.upd s (SZ.v i) v))
-}
-
-
-inline_for_extraction
-fn free
-    (#elt: Type)
-    (a: array elt)
-    (#s: Ghost.erased (Seq.seq elt))
-requires
-  pts_to a s ** pure (is_full_array a)
-ensures
-  emp
-{
-  unfold (pts_to a s);
-  H.free a;
-}
-
-
-let share #a arr #s #p = H.share arr #(raise_seq s) #p
-
-
-ghost
-fn gather
-  (#a:Type)
-  (arr:array a)
-  (#s0 #s1:Ghost.erased (Seq.seq a))
-  (#p0 #p1:perm)
-  requires pts_to arr #p0 s0 ** pts_to arr #p1 s1
-  ensures pts_to arr #(p0 +. p1) s0 ** pure (s0 == s1)
-{
-  unfold (pts_to arr #p0 s0);
-  unfold (pts_to arr #p1 s1);
-  H.gather arr #_ #_ #p0 #p1;
-  fold (pts_to arr #(p0 +. p1) s0);
-}
-
-
-let pts_to_range
-  (#a:Type)
-  ([@@@mkey] x:array a)
-  ([@@@mkey] i : nat)
-  (j : nat)
-  (#[exact (`1.0R)] p:perm)
-  (s : Seq.seq a)
-: slprop
-= H.pts_to_range x i j #p (raise_seq s)
+let pts_to_range x = H.pts_to_range x
 
 let pts_to_range_timeless _ _ _ _ _ = ()
 
+let pts_to_range_prop a = H.pts_to_range_prop a
 
-ghost
-fn pts_to_range_prop
-  (#elt: Type)
-  (a: array elt)
-  (#i #j: nat)
-  (#p: perm)
-  (#s: Seq.seq elt)
-requires
-  pts_to_range a i j #p s
-ensures
-  pts_to_range a i j #p s **
-  pure (
-      (i <= j /\ j <= length a /\ Seq.length s == (j - i))
-  )
-{
-  unfold (pts_to_range a i j #p s);
-  H.pts_to_range_prop a #i #j #p #(raise_seq s);
-  fold (pts_to_range a i j #p s);
-}
+let pts_to_range_intro a = H.pts_to_range_intro a
+let pts_to_range_elim a = H.pts_to_range_elim a
 
-let pts_to_range_intro a p s = H.pts_to_range_intro a p (raise_seq s)
-let pts_to_range_elim a p s = H.pts_to_range_elim a p (raise_seq s)
+let pts_to_range_split a = H.pts_to_range_split a
+let pts_to_range_join a = H.pts_to_range_join a
 
+inline_for_extraction let pts_to_range_index a = H.pts_to_range_index a
+inline_for_extraction let pts_to_range_upd a = H.pts_to_range_upd a
 
-ghost
-fn pts_to_range_split
-  (#elt: Type0)
-  (a: array elt)
-  (i m j: nat)
-  (#p: perm)
-  (#s: Seq.seq elt)
-  requires
-    pts_to_range a i j #p s **
-    pure (i <= m /\ m <= j)
-  ensures
-    exists* s1 s2.
-      pts_to_range a i m #p s1 **
-      pts_to_range a m j #p s2 **
-      pure (
-        i <= m /\ m <= j /\ j <= length a /\
-        eq2 #int (Seq.length s) (j - i) /\
-        s1 == Seq.slice s 0 (m - i) /\
-        s2 == Seq.slice s (m - i) (Seq.length s) /\
-        s == Seq.append s1 s2
-      )
-{
-  unfold (pts_to_range a i j #p s);
-  H.pts_to_range_split a i m j #p #(raise_seq s);
-  with s1 s2. _;
-  fold (pts_to_range a i m #p (downgrade_seq s1));
-  fold (pts_to_range a m j #p (downgrade_seq s2));  
-  let s1 = downgrade_seq s1;
-  let s2 = downgrade_seq s2;
-  assert pure ( 
-    s1 `Seq.equal` Seq.slice s 0 (m - i) /\
-    s2 `Seq.equal` Seq.slice s (m - i) (Seq.length s) /\
-    s `Seq.equal` Seq.append s1 s2
-  )
-}
-
-
-
-ghost
-fn pts_to_range_join
-  (#elt: Type0)
-  (a: array elt)
-  (i m j: nat)
-  (#p: perm)
-  (#s1 #s2: Seq.seq elt)
-requires
-  pts_to_range a i m #p s1 **
-  pts_to_range a m j #p s2
-ensures
-  pts_to_range a i j #p (s1 `Seq.append` s2)
-{
-  unfold (pts_to_range a i m #p s1);
-  unfold (pts_to_range a m j #p s2);
-  H.pts_to_range_join a i m j;
-  assert pure (
-    Seq.append (raise_seq s1) (raise_seq s2) `Seq.equal`
-    raise_seq (s1 `Seq.append` s2)
-  );
-  fold (pts_to_range a i j #p (s1 `Seq.append` s2));
-}
-
-
-
-inline_for_extraction
-fn pts_to_range_index
-  (#t: Type)
-  (a: array t)
-  (i: SZ.t)
-  (#l: Ghost.erased nat{l <= SZ.v i})
-  (#r: Ghost.erased nat{SZ.v i < r})
-  (#s: Ghost.erased (Seq.seq t))
-  (#p: perm)
-requires
-  pts_to_range a l r #p s
-  returns res:t
-ensures 
-  pts_to_range a l r #p s **
-  pure (eq2 #int (Seq.length s) (r - l) /\
-        res == Seq.index s (SZ.v i - l))
-{
-  unfold (pts_to_range a l r #p s);
-  let res = H.pts_to_range_index a i;
-  fold (pts_to_range a l r #p s);
-  U.downgrade_val res
-}
-
-
-
-inline_for_extraction
-fn pts_to_range_upd
-  (#t: Type)
-  (a: array t)
-  (i: SZ.t)
-  (v: t)
-  (#l: Ghost.erased nat{l <= SZ.v i})
-  (#r: Ghost.erased nat{SZ.v i < r})
-  (#s0: Ghost.erased (Seq.seq t))
-  requires pts_to_range a l r s0
-  ensures
-    exists* s.
-      pts_to_range a l r s **
-      pure(
-        eq2 #int (Seq.length s0) (r - l) /\
-        s == Seq.upd s0 (SZ.v i - l) v
-      )
-{
-  unfold (pts_to_range a l r s0);
-  H.pts_to_range_upd a i (U.raise_val v);
-  with s. _;
-  assert (
-    pure (
-      s `Seq.equal` (raise_seq (Seq.upd s0 (SZ.v i - l) v))
-    )
-  );
-  fold (pts_to_range a l r (Seq.upd s0 (SZ.v i - l) v));
-}
-
+let pts_to_range_share arr = H.pts_to_range_share arr
+let pts_to_range_gather arr = H.pts_to_range_gather arr
 
 let with_pre (pre:slprop) (#a:Type) (#post:a -> slprop)(m:stt a emp post)
 : stt a pre (fun v -> pre ** post v)
@@ -593,38 +139,6 @@ fn free_with_post (#a:Type u#0) (arr:array a) (post:slprop)
   ensures post
 {
   free arr  
-}
-
-ghost
-fn pts_to_range_share
-  (#a:Type)
-  (arr:array a)
-  (#l #r: nat)
-  (#s:Seq.seq a)
-  (#p:perm)
-      requires pts_to_range arr l r #p s
-      ensures pts_to_range arr l r #(p /. 2.0R) s ** pts_to_range arr l r #(p /. 2.0R) s
-{
-  unfold (pts_to_range arr l r #p s);
-  H.pts_to_range_share arr;
-  fold (pts_to_range arr l r #(p /. 2.0R) s);
-  fold (pts_to_range arr l r #(p /. 2.0R) s);
-}
-
-ghost
-fn pts_to_range_gather
-  (#a:Type)
-  (arr:array a)
-  (#l #r: nat)
-  (#s0 #s1: Seq.seq a)
-  (#p0 #p1:perm)
-      requires pts_to_range arr l r #p0 s0 ** pts_to_range arr l r #p1 s1
-      ensures pts_to_range arr l r #(p0 +. p1) s0 ** pure (s0 == s1)
-{
-  unfold (pts_to_range arr l r #p0 s0);
-  unfold (pts_to_range arr l r #p1 s1);
-  H.pts_to_range_gather arr;
-  fold (pts_to_range arr l r #(p0 +. p1) s0)
 }
 
 (* this is universe-polymorphic in ret_t; so can't define it in Pulse yet *)
