pulse/lib/pulse/lib/Pulse.Lib.HigherReference.fst
@@ -19,9 +19,9 @@ module Pulse.Lib.HigherReference
 open Pulse.Lib.Core
 module A = Pulse.Lib.HigherArray
 
-let ref (a:Type u#1) = A.array a
+let ref a = A.array a
 
-let null (#a:Type u#1) : ref a = A.null
+let null #a : ref a = A.null
 
 let is_null #a (r : ref a)
   : b:bool{b <==> r == null #a}
@@ -34,13 +34,13 @@ let upd_singleton #a (x y: a) :
       [SMTPat (Seq.upd (singleton x) 0 y)] =
   assert Seq.equal (Seq.upd (singleton x) 0 y) (singleton y)
 
-let pts_to (#a:Type) (r:ref a) (#[T.exact (`1.0R)] p:perm) (n:a)
+let pts_to (#a: Type u#a) (r:ref a) (#[T.exact (`1.0R)] p:perm) (n:a)
 = A.pts_to r #p (singleton n)
 let pts_to_timeless _ _ _ = ()
 
 let is_full_ref = A.is_full_array
 
-fn alloc (#a:Type u#1) (x:a)
+fn alloc u#a (#a: Type u#a) {| small_type u#a |} (x:a)
   returns r:ref a
   ensures pts_to r x
   ensures pure (is_full_ref r)
@@ -50,7 +50,7 @@ fn alloc (#a:Type u#1) (x:a)
   r
 }
 
-fn read (#a:Type u#1) (r:ref a) (#n:erased a) (#p:perm)
+fn read u#a (#a: Type u#a) (r:ref a) (#n:erased a) (#p:perm)
   preserves r |-> Frac p n
   returns  x : a
   ensures  rewrites_to x n
@@ -63,7 +63,7 @@ fn read (#a:Type u#1) (r:ref a) (#n:erased a) (#p:perm)
 
 let ( ! ) #a = read #a
 
-fn write (#a:Type u#1) (r:ref a) (x:a) (#n:erased a)
+fn write u#a (#a: Type u#a) (r:ref a) (x:a) (#n:erased a)
   requires r |-> n
   ensures  r |-> x
 {
@@ -75,7 +75,7 @@ fn write (#a:Type u#1) (r:ref a) (x:a) (#n:erased a)
 let ( := ) #a = write #a
 
 
-fn free #a (r:ref a) (#n:erased a)
+fn free u#a (#a: Type u#a) (r:ref a) (#n:erased a)
   requires pts_to r #1.0R n
   requires pure (is_full_ref r)
 {
@@ -84,7 +84,7 @@ fn free #a (r:ref a) (#n:erased a)
 }
 
 ghost
-fn share #a (r:ref a) (#v:erased a) (#p:perm)
+fn share u#a (#a: Type u#a) (r:ref a) (#v:erased a) (#p:perm)
   requires pts_to r #p v
   ensures pts_to r #(p /. 2.0R) v ** pts_to r #(p /. 2.0R) v
 {
@@ -95,7 +95,7 @@ fn share #a (r:ref a) (#v:erased a) (#p:perm)
 }
 
 ghost
-fn gather #a (r:ref a) (#x0 #x1:erased a) (#p0 #p1:perm)
+fn gather u#a (#a: Type u#a) (r:ref a) (#x0 #x1:erased a) (#p0 #p1:perm)
   requires pts_to r #p0 x0 ** pts_to r #p1 x1
   ensures pts_to r #(p0 +. p1) x0 ** pure (x0 == x1)
 { 
@@ -107,7 +107,7 @@ fn gather #a (r:ref a) (#x0 #x1:erased a) (#p0 #p1:perm)
 
 (* this is universe-polymorphic in ret_t; so can't define it in Pulse yet *)
 
-fn alloc_with_frame #a (init: a) pre
+fn alloc_with_frame u#a (#a: Type u#a) {| small_type u#a |} (init: a) pre
   requires pre
   returns r: ref a
   ensures (pre ** pts_to r init) ** pure (is_full_ref r)
@@ -115,7 +115,7 @@ fn alloc_with_frame #a (init: a) pre
   alloc init
 }
 
-fn free_with_frame #a (r:ref a) (frame:slprop)
+fn free_with_frame u#a (#a: Type u#a) (r:ref a) (frame:slprop)
   requires ((frame ** (exists* (x: a). pts_to r x)) ** pure (is_full_ref r))
   ensures frame
 {
@@ -123,12 +123,12 @@ fn free_with_frame #a (r:ref a) (frame:slprop)
 }
 
 let with_local
-    (#a:Type u#1)
+    (#a: Type u#a) {| small_type u#a |}
     (init:a)
     (#pre:slprop)
-    (#ret_t:Type u#a)
+    (#ret_t:Type u#b)
     (#post:ret_t -> slprop) 
-    (body: (r:ref a -> stt ret_t (pre ** pts_to r init) (fun v -> post v ** (exists* (x:a). pts_to r x))))
+    (body: (r:ref a -> stt ret_t (pre ** pts_to u#a r init) (fun v -> post v ** (exists* (x:a). pts_to u#a r x))))
 = bind_stt (alloc_with_frame init pre) fun r ->
   bind_stt (frame_stt (pure (is_full_ref r)) (body r)) fun ret ->
   bind_stt (free_with_frame r _) fun _ ->
@@ -137,7 +137,7 @@ let with_local
 
 ghost
 fn pts_to_injective_eq
-    (#a:Type)
+    u#a (#a: Type u#a)
     (#p0 #p1:perm)
     (#v0 #v1:a)
     (r:ref a)
@@ -153,7 +153,7 @@ fn pts_to_injective_eq
 
 
 ghost
-fn pts_to_perm_bound (#a:_) (#p:_) (r:ref a) (#v:a)
+fn pts_to_perm_bound u#a (#a: Type u#a) (#p:_) (r:ref a) (#v:a)
   requires pts_to r #p v
   ensures pts_to r #p v ** pure (p <=. 1.0R)
 {
@@ -163,7 +163,7 @@ fn pts_to_perm_bound (#a:_) (#p:_) (r:ref a) (#v:a)
 }
 
 ghost
-fn pts_to_not_null (#a:_) (#p:_) (r:ref a) (#v:a)
+fn pts_to_not_null u#a (#a: Type u#a) (#p:_) (r:ref a) (#v:a)
   preserves r |-> Frac p v
   ensures  pure (not (is_null #a r))
 {
@@ -175,7 +175,7 @@ fn pts_to_not_null (#a:_) (#p:_) (r:ref a) (#v:a)
 let to_array_ghost r = r
 
 unobservable
-fn to_array #a (r: ref a) #p (#v: erased a)
+fn to_array u#a (#a: Type u#a) (r: ref a) #p (#v: erased a)
   requires r |-> Frac p v
   returns arr: array a
   ensures rewrites_to arr (to_array_ghost r)
@@ -189,7 +189,7 @@ fn to_array #a (r: ref a) #p (#v: erased a)
 }
 
 ghost
-fn return_to_array #a (r: ref a) #p (#v: Seq.seq a)
+fn return_to_array u#a (#a: Type u#a) (r: ref a) #p (#v: Seq.seq a)
   requires to_array_ghost r |-> Frac p v
   requires pure (length (to_array_ghost r) == 1)
   returns _: squash (Seq.length v == 1)
@@ -203,7 +203,7 @@ fn return_to_array #a (r: ref a) #p (#v: Seq.seq a)
 let array_at_ghost arr i = gsub arr i (i+1)
 
 unobservable
-fn array_at #a (arr: array a) (i: SizeT.t) #p (#v: erased (Seq.seq a) { SizeT.v i < length arr /\ length arr == Seq.length v }) #mask
+fn array_at u#a (#a: Type u#a) (arr: array a) (i: SizeT.t) #p (#v: erased (Seq.seq a) { SizeT.v i < length arr /\ length arr == Seq.length v }) #mask
   requires pts_to_mask arr #p v mask
   requires pure (mask (SizeT.v i))
   returns r: ref a
@@ -220,7 +220,7 @@ fn array_at #a (arr: array a) (i: SizeT.t) #p (#v: erased (Seq.seq a) { SizeT.v 
 }
 
 ghost
-fn return_array_at (#a: Type u#1) (arr: array a) (i: nat) (#p: perm) (#v: a) (#v': Seq.seq a { i < length arr /\ length arr == Seq.length v' }) (#mask: nat->prop)
+fn return_array_at u#a (#a: Type u#a) (arr: array a) (i: nat) (#p: perm) (#v: a) (#v': Seq.seq a { i < length arr /\ length arr == Seq.length v' }) (#mask: nat->prop)
   requires array_at_ghost arr i |-> Frac p v
   requires pts_to_mask arr #p v' mask
   requires pure (~(mask i))
