pulse/lib/pulse/lib/Pulse.Lib.HigherReference.fsti
@@ -22,74 +22,75 @@ open PulseCore.FractionalPermission
 open FStar.Ghost
 open Pulse.Class.PtsTo
 open Pulse.Lib.HigherArray
+open Pulse.Lib.SmallType
 module T = FStar.Tactics
-val ref ([@@@unused]a:Type u#1) : Type u#0
+val ref ([@@@unused]a:Type) : Type0
 
-val null (#a:Type u#1) : ref a
+val null #a : ref a
 
 val is_null #a (r : ref a) : b:bool{b <==> r == null #a}
 
-val pts_to (#a:Type) ([@@@mkey]r:ref a) (#[T.exact (`1.0R)] p:perm) (n:a) : slprop
+val pts_to (#a:Type u#a) ([@@@mkey]r:ref a) (#[T.exact (`1.0R)] p:perm) (n:a) : slprop
 
 [@@pulse_unfold]
-instance has_pts_to_ref (a:Type) : has_pts_to (ref a) a = {
+instance has_pts_to_ref (a:Type u#a) : has_pts_to (ref a) a = {
   pts_to = (fun r #f v -> pts_to r #f v);
 }
 
-val pts_to_timeless (#a:Type) (r:ref a) (p:perm) (n:a)
+val pts_to_timeless (#a: Type u#a) (r:ref a) (p:perm) (n:a)
   : Lemma (timeless (pts_to r #p n))
           [SMTPat (timeless (pts_to r #p n))]
 
 val is_full_ref #a (x: ref a) : prop
 
 [@@deprecated "HigherReference.alloc is unsound; only use for model implementations"]
-fn alloc (#a:Type) (x:a)
+fn alloc u#a (#a: Type u#a) {| small_type u#a |} (x:a)
   returns  r : ref a
   ensures  r |-> x
   ensures  pure (is_full_ref r)
   
-fn read (#a:Type) (r:ref a) (#n:erased a) (#p:perm)
+fn read u#a (#a: Type u#a) (r:ref a) (#n:erased a) (#p:perm)
   preserves r |-> Frac p n
   returns  x : a
   ensures  rewrites_to x n
 
 (* alias for read *)
-fn ( ! ) (#a:Type) (r:ref a) (#n:erased a) (#p:perm)
+fn ( ! ) u#a (#a: Type u#a) (r:ref a) (#n:erased a) (#p:perm)
   preserves r |-> Frac p n
   returns  x : a
   ensures  rewrites_to x n
 
-fn write (#a:Type) (r:ref a) (x:a) (#n:erased a)
+fn write u#a (#a: Type u#a) (r:ref a) (x:a) (#n:erased a)
   requires r |-> n
   ensures  r |-> x
 
 (* alias for write *)
-fn ( := ) (#a:Type) (r:ref a) (x:a) (#n:erased a)
+fn ( := ) u#a (#a: Type u#a) (r:ref a) (x:a) (#n:erased a)
   requires r |-> n
   ensures  r |-> x
 
 [@@deprecated "HigherReference.free is unsound; only use for model implementations"]
-fn free (#a:Type) (r:ref a) (#n:erased a)
+fn free u#a (#a: Type u#a) (r:ref a) (#n:erased a)
   requires pts_to r n
   requires pure (is_full_ref r)
 
 ghost
-fn share (#a:Type) (r:ref a) (#v:erased a) (#p:perm)
+fn share u#a (#a: Type u#a) (r:ref a) (#v:erased a) (#p:perm)
   requires r |-> Frac p v
   ensures  (r |-> Frac (p /. 2.0R) v) **
            (r |-> Frac (p /. 2.0R) v)
 
 [@@allow_ambiguous]
 ghost
-fn gather (#a:Type) (r:ref a) (#x0 #x1:erased a) (#p0 #p1:perm)
+fn gather u#a (#a: Type u#a) (r:ref a) (#x0 #x1:erased a) (#p0 #p1:perm)
   requires (r |-> Frac p0 x0) ** (r |-> Frac p1 x1)
   ensures  (r |-> Frac (p0 +. p1) x0) ** pure (x0 == x1)
 
 val with_local
-  (#a:Type u#1)
+  (#a:Type u#a) {| small_type u#a |}
   (init:a)
   (#pre:slprop)
-  (#ret_t:Type)
+  (#ret_t:Type u#b)
   (#post:ret_t -> slprop)
   (body:(r:ref a) -> stt ret_t (pre ** pts_to r init)
                                (fun v -> post v ** (exists* (x:a). pts_to r x)))
@@ -97,7 +98,7 @@ val with_local
 
 [@@allow_ambiguous]
 ghost
-fn pts_to_injective_eq (#a:_)
+fn pts_to_injective_eq u#a (#a: Type u#a)
                         (#p #q:_)
                         (#v0 #v1:a)
                         (r:ref a)
@@ -105,19 +106,19 @@ fn pts_to_injective_eq (#a:_)
   ensures   pure (v0 == v1)
 
 ghost
-fn pts_to_perm_bound (#a:_) (#p:_) (r:ref a) (#v:a)
+fn pts_to_perm_bound u#a (#a: Type u#a) (#p:_) (r:ref a) (#v:a)
   preserves r |-> Frac p v
   ensures   pure (p <=. 1.0R)
 
 ghost
-fn pts_to_not_null (#a:_) (#p:_) (r:ref a) (#v:a)
+fn pts_to_not_null u#a (#a: Type u#a) (#p:_) (r:ref a) (#v:a)
   preserves r |-> Frac p v
   ensures  pure (not (is_null #a r))
 
 val to_array_ghost #a (r: ref a) : GTot (array a)
 
 unobservable
-fn to_array #a (r: ref a) #p (#v: erased a)
+fn to_array u#a (#a: Type u#a) (r: ref a) #p (#v: erased a)
   requires r |-> Frac p v
   returns arr: array a
   ensures rewrites_to arr (to_array_ghost r)
@@ -125,16 +126,16 @@ fn to_array #a (r: ref a) #p (#v: erased a)
   ensures pure (length arr == 1)
 
 ghost
-fn return_to_array #a (r: ref a) #p (#v: Seq.seq a)
+fn return_to_array u#a (#a: Type u#a) (r: ref a) #p (#v: Seq.seq a)
   requires to_array_ghost r |-> Frac p v
   requires pure (length (to_array_ghost r) == 1)
   returns _: squash (Seq.length v == 1)
   ensures r |-> Frac p (Seq.index v 0)
 
-val array_at_ghost #a (arr: array a) (i: nat { i < length arr }) : GTot (r:ref a { to_array_ghost r == gsub arr i (i+1) })
+val array_at_ghost (#a: Type u#a) (arr: array a) (i: nat { i < length arr }) : GTot (r:ref a { to_array_ghost r == gsub arr i (i+1) })
 
 unobservable
-fn array_at #a (arr: array a) (i: SizeT.t) #p (#v: erased (Seq.seq a) { SizeT.v i < length arr /\ length arr == Seq.length v }) #mask
+fn array_at u#a (#a: Type u#a) (arr: array a) (i: SizeT.t) #p (#v: erased (Seq.seq a) { SizeT.v i < length arr /\ length arr == Seq.length v }) #mask
   requires pts_to_mask arr #p v mask
   requires pure (mask (SizeT.v i))
   returns r: ref a
@@ -143,7 +144,7 @@ fn array_at #a (arr: array a) (i: SizeT.t) #p (#v: erased (Seq.seq a) { SizeT.v 
   ensures pts_to_mask arr #p v (fun k -> mask k /\ k <> SizeT.v i)
 
 ghost
-fn return_array_at (#a: Type u#1) (arr: array a) (i: nat) (#p: perm) (#v: a) (#v': Seq.seq a { i < length arr /\ length arr == Seq.length v' }) (#mask: nat->prop)
+fn return_array_at u#a (#a: Type u#a) (arr: array a) (i: nat) (#p: perm) (#v: a) (#v': Seq.seq a { i < length arr /\ length arr == Seq.length v' }) (#mask: nat->prop)
   requires array_at_ghost arr i |-> Frac p v
   requires pts_to_mask arr #p v' mask
   requires pure (~(mask i))
