pulse/lib/pulse/lib/Pulse.Lib.Reference.fst
@@ -20,9 +20,8 @@ open Pulse.Lib.Core
 open Pulse.Main
 module H = Pulse.Lib.HigherReference
 friend Pulse.Lib.Array.Core
-module U = Pulse.Lib.Raise
 inline_for_extraction
-let ref a = H.ref (U.raise_t a)
+let ref a = H.ref a
 
 inline_for_extraction
 let null (#a:Type u#0) : ref a = H.null
@@ -32,122 +31,21 @@ let is_null #a (r : ref a)
   : b:bool{b <==> r == null #a}
 = H.is_null r
 
-let pts_to
-    (#a:Type u#0)
-    (r:ref a)
-    (#p:perm)
-    (v:a)
-  = H.pts_to r #p (U.raise_val v)
+let pts_to r = H.pts_to r
 
-let pts_to_timeless r p x = H.pts_to_timeless r p (U.raise_val x)
+let pts_to_timeless r p x = ()
 
 let is_full_ref r = H.is_full_ref r
 
-inline_for_extraction
-fn alloc (#a:Type u#0) (v:a)
-  returns r:ref a
-  ensures pts_to r v
-  ensures  pure (is_full_ref r)
-{
-  let r = H.alloc (U.raise_val v);
-  fold (pts_to r #1.0R v);
-  r
-}
+inline_for_extraction let alloc v = H.alloc v
+inline_for_extraction let read r = H.read r
+inline_for_extraction let op_Bang = read
+inline_for_extraction let write r = H.write r
+inline_for_extraction let op_Colon_Equals = write
+inline_for_extraction let free r = H.free r
 
-
-
-inline_for_extraction
-fn read
-  (#a:Type)
-  (r:ref a)
-  (#n:erased a)
-  (#p:perm)
-  preserves pts_to r #p n
-  returns x:a
-  ensures rewrites_to x n
-{
-  unfold (pts_to r #p n);
-  let k = H.( !r );
-  fold (pts_to r #p n);
-  U.downgrade_val k
-}
-
-inline_for_extraction
-let op_Bang = read
-
-inline_for_extraction
-fn write
-  (#a:Type)
-  (r:ref a)
-  (x:a)
-  (#n:erased a)
-  requires pts_to r #1.0R n
-  ensures pts_to r #1.0R x
-{
-  unfold (pts_to r #1.0R n);
-  H.(r := (U.raise_val x));
-  fold (pts_to r #1.0R x)
-}
-
-inline_for_extraction
-let op_Colon_Equals = write
-
-inline_for_extraction
-fn free #a (r:ref a) (#n:erased a)
-  requires pts_to r #1.0R n
-  requires pure (is_full_ref r)
-{
-  unfold (pts_to r #1.0R n);
-  H.free r;
-}
-
-
-
-ghost
-fn share (#a:Type) (r:ref a) (#v:erased a) (#p:perm)
-  requires pts_to r #p v
-  ensures pts_to r #(p /. 2.0R) v ** pts_to r #(p /. 2.0R) v
-{
-  unfold pts_to r #p v;
-  H.share r;
-  fold pts_to r #(p /. 2.0R) v;
-  fold pts_to r #(p /. 2.0R) v
-}
-
-
-
-ghost
-fn raise_inj (a:Type u#0) (x0 x1:a)
-  requires pure (U.raise_val u#0 u#1 x0 == U.raise_val u#0 u#1 x1)
-  ensures pure (x0 == x1)
-{
-  assert pure (U.downgrade_val (U.raise_val u#0 u#1 x0) == x0);
-  assert pure (U.downgrade_val (U.raise_val u#0 u#1 x1) == x1);
-}
-
-
-
-ghost
-fn gather (#a:Type) (r:ref a) (#x0 #x1:erased a) (#p0 #p1:perm)
-  requires pts_to r #p0 x0 ** pts_to r #p1 x1
-  ensures pts_to r #(p0 +. p1) x0 ** pure (x0 == x1)
-{
-  unfold pts_to r #p0 x0;
-  unfold pts_to r #p1 x1;
-  H.gather r;
-  fold (pts_to r #(p1 +. p0) x0);
-  raise_inj a x0 x1;
-}
-
-
-
-fn
-raise_exists (#a:Type u#0) (frame:slprop) (p: U.raise_t u#0 u#1 a -> slprop)
-  requires frame ** (exists* (x:a). p (U.raise_val x))
-  ensures frame ** (exists* (x:U.raise_t a). p x)
-{
-  ()
-}
+let share r = H.share r
+let gather r = H.gather r
 
 
 let with_local
@@ -157,70 +55,14 @@ let with_local
     (#ret_t:Type)
     (#post:ret_t -> slprop)
     (body:(r:ref a) -> stt ret_t (pre ** pts_to r init)
-                                 (fun v -> post v ** op_exists_Star (pts_to r #1.0R)))
+                                 (fun v -> post v ** (exists* v. pts_to r v)))
 : stt ret_t pre post
-= let body (r:H.ref (U.raise_t a))
-    : stt ret_t (pre ** H.pts_to r #1.0R (U.raise_val init))
-                (fun v -> post v ** (exists* (x:U.raise_t a). H.pts_to r #1.0R x)) 
-    = let m
-        : stt ret_t (pre ** H.pts_to r #1.0R (U.raise_val init))
-                    (fun v -> post v ** (exists* (x:a). H.pts_to r #1.0R (U.raise_val x)))
-        = body r
-      in
-      let m0 (v:ret_t)
-        : stt ret_t 
-            (post v ** (exists* (x:a). H.pts_to r #1.0R (U.raise_val x)))
-            (fun v -> post v ** (exists* (x:U.raise_t a). H.pts_to r #1.0R x))
-        = bind_stt (raise_exists (post v) (H.pts_to r #1.0R))
-                   (fun _ -> return_stt_noeq v (fun v -> post v ** (exists* (x:U.raise_t a). H.pts_to r #1.0R x)))
-      in
-      bind_stt m m0
-  in
-  H.with_local (U.raise_val init) body
+= H.with_local init #pre #ret_t #post (fun r -> body r)
 
 
-ghost
-fn pts_to_injective_eq
-  (#a:Type0)
-  (#p #q:perm)
-  (#v0 #v1:a)
-  (r:ref a)
-requires
-  pts_to r #p v0 ** pts_to r #q v1
-ensures
-  pts_to r #p v0 ** pts_to r #q v1 ** pure (v0 == v1)
-{
-  unfold pts_to r #p v0;
-  unfold pts_to r #q v1;
-  H.pts_to_injective_eq r;
-  fold pts_to r #p v0;
-  fold pts_to r #q v1;
-  raise_inj _ v0 v1;
-}
-
-
-
-ghost
-fn pts_to_perm_bound (#a:_) (#p:_) (r:ref a) (#v:a)
-  requires pts_to r #p v
-  ensures pts_to r #p v ** pure (p <=. 1.0R)
-{
-  unfold pts_to r #p v;
-  H.pts_to_perm_bound r;
-  fold pts_to r #p v;
-}
-
-
-ghost
-fn pts_to_not_null (#a:_) (#p:_) (r:ref a) (#v:a)
-  preserves r |-> Frac p v
-  ensures  pure (not (is_null #a r))
-{
-  unfold pts_to r #p v;
-  let res = H.pts_to_not_null r;
-  fold pts_to r #p v;
-  res
-}
+let pts_to_injective_eq r = H.pts_to_injective_eq r
+let pts_to_perm_bound r = H.pts_to_perm_bound r
+let pts_to_not_null r = H.pts_to_not_null r
 
 fn replace (#a:Type0) (r:ref a) (x:a) (#v:erased a)
   requires pts_to r v
@@ -233,63 +75,9 @@ fn replace (#a:Type0) (r:ref a) (x:a) (#v:erased a)
 }
 
 let to_array_ghost r = H.to_array_ghost r
-
-inline_for_extraction
-unobservable
-fn to_array #a (r: ref a) #p (#v: erased a)
-  requires r |-> Frac p v
-  returns arr: array a
-  ensures rewrites_to arr (to_array_ghost r)
-  ensures arr |-> Frac p (seq![reveal v])
-  ensures pure (length arr == 1)
-{
-  unfold pts_to r #p v;
-  let res = H.to_array r;
-  assert pure (raise_seq seq![reveal v] `Seq.equal` seq![U.raise_val (reveal v)]);
-  fold Pulse.Lib.Array.Core.pts_to res #p seq![reveal v];
-  res;
-}
-
-ghost
-fn return_to_array #a (r: ref a) #p (#v: Seq.seq a)
-  requires to_array_ghost r |-> Frac p v
-  requires pure (length (to_array_ghost r) == 1)
-  returns _: squash (Seq.length v == 1)
-  ensures r |-> Frac p (Seq.index v 0)
-{
-  unfold Pulse.Lib.Array.Core.pts_to (to_array_ghost r) #p v;
-  H.return_to_array r #p #(raise_seq v);
-  fold pts_to r #p (Seq.index v 0);
-}
+inline_for_extraction let to_array r = H.to_array r
+let return_to_array r = H.return_to_array r
 
 let array_at_ghost arr i = H.array_at_ghost arr i
-
-inline_for_extraction
-unobservable
-fn array_at #a (arr: array a) (i: SizeT.t) #p (#v: erased (Seq.seq a) { SizeT.v i < length arr /\ length arr == Seq.length v }) #mask
-  requires pts_to_mask arr #p v mask
-  requires pure (mask (SizeT.v i))
-  returns r: ref a
-  ensures rewrites_to r (array_at_ghost arr (SizeT.v i))
-  ensures r |-> Frac p (Seq.index v (SizeT.v i))
-  ensures pts_to_mask arr #p v (fun k -> mask k /\ k <> SizeT.v i)
-{
-  unfold pts_to_mask arr #p v mask;
-  let res = H.array_at arr i;
-  fold pts_to_mask arr #p v (fun k -> mask k /\ k <> SizeT.v i);
-  fold pts_to (H.array_at_ghost arr (SizeT.v i)) #p (Seq.Base.index v (SizeT.v i));
-  res
-}
-
-ghost
-fn return_array_at #a (arr: array a) (i: nat) (#p: perm) (#v: a) (#v': Seq.seq a { i < length arr /\ length arr == Seq.length v' }) (#mask: nat->prop)
-  requires array_at_ghost arr i |-> Frac p v
-  requires pts_to_mask arr #p v' mask
-  requires pure (~(mask i))
-  ensures pts_to_mask arr #p (Seq.upd v' i v) (fun k -> mask k \/ k == i)
-{
-  unfold pts_to (array_at_ghost arr i) #p v;
-  H.return_array_at arr i;
-  assert pure (raise_seq (Seq.Base.upd v' i v) `Seq.equal` Seq.upd (raise_seq v') i (U.raise_val v));
-  fold pts_to_mask arr #p (Seq.upd v' i v) (fun k -> mask k \/ k == i);
-}
+inline_for_extraction let array_at arr = H.array_at arr
+let return_array_at arr = H.return_array_at arr
