pulse/lib/pulse/lib/Pulse.Lib.HigherArray.Core.fsti
@@ -23,10 +23,11 @@ open Pulse.Class.PtsTo
 open PulseCore.FractionalPermission
 open FStar.Ghost
 module SZ = FStar.SizeT
+open Pulse.Lib.SmallType
 
 [@@erasable] val base_t : Type0
 
-val array ([@@@unused] a:Type u#1) : Type u#0
+val array ([@@@unused] a:Type u#a) : Type u#0
 
 val length (#a:Type) (x:array a) : Ghost nat (requires True) (ensures SZ.fits)
 val base_of #t (a: array t) : base_t
@@ -41,64 +42,64 @@ val is_full_array (#a:Type) (x:array a) : prop
 val null #a : array a
 val is_null #a (r: array a) : b:bool {b <==> r == null #a}
 
-val pts_to_mask #t ([@@@mkey] a: array t) (#[full_default()] f: perm) (v: erased (Seq.seq t)) (mask: nat -> prop) : slprop
+val pts_to_mask (#t: Type u#a) ([@@@mkey] a: array t) (#[full_default()] f: perm) (v: erased (Seq.seq t)) (mask: nat -> prop) : slprop
 
-val pts_to_mask_timeless (#a:Type) (x:array a) (p:perm) (s:Seq.seq a) mask
+val pts_to_mask_timeless (#a:Type u#a) (x:array a) (p:perm) (s:Seq.seq a) mask
   : Lemma (timeless (pts_to_mask x #p s mask))
           [SMTPat (timeless (pts_to_mask x #p s mask))]
 
 ghost
-fn pts_to_mask_len #t (a:array t) (#p:perm) (#x:Seq.seq t) #mask
+fn pts_to_mask_len u#a (#t: Type u#a) (a:array t) (#p:perm) (#x:Seq.seq t) #mask
   preserves pts_to_mask a #p x mask
   ensures pure (length a == Seq.length x)
 
 ghost
-fn pts_to_mask_perm_bound #t (arr: array t) #p (#s:Seq.seq t) #mask
+fn pts_to_mask_perm_bound u#a (#t: Type u#a) (arr: array t) #p (#s:Seq.seq t) #mask
   preserves pts_to_mask arr #p s mask
   requires pure (exists (i: nat). i < Seq.length s /\ mask i)
   ensures pure (p <=. 1.0R)
 
 ghost
-fn pts_to_mask_not_null #a #p (r:array a) (#v:Seq.seq a) #mask
+fn pts_to_mask_not_null u#a (#a: Type u#a) #p (r:array a) (#v:Seq.seq a) #mask
   preserves pts_to_mask r #p v mask
   ensures pure (not (is_null r))
 
-ghost fn mask_vext #t (arr: array t) #f #v v' #mask
+ghost fn mask_vext u#a (#t: Type u#a) (arr: array t) #f #v v' #mask
   requires pts_to_mask arr #f v mask
   requires pure (Seq.length v' == Seq.length v /\
     (forall (i: nat). mask i /\ i < Seq.length v ==> Seq.index v i == Seq.index v' i))
   ensures pts_to_mask arr #f v' mask
 
-ghost fn mask_mext #t (arr: array t) #f #v #mask (mask': nat -> prop)
+ghost fn mask_mext u#a (#t: Type u#a) (arr: array t) #f #v #mask (mask': nat -> prop)
   requires pts_to_mask arr #f v mask
   requires pure (forall (i: nat). i < Seq.length v ==> (mask i <==> mask' i))
   ensures pts_to_mask arr #f v mask'
 
-ghost fn mask_ext #t (arr: array t) #f #v #mask v' (mask': nat -> prop)
+ghost fn mask_ext u#a (#t: Type u#a) (arr: array t) #f #v #mask v' (mask': nat -> prop)
   requires pts_to_mask arr #f v mask
   requires pure (forall (i: nat). i < Seq.length v ==> (mask i <==> mask' i))
   requires pure (Seq.length v' == Seq.length v /\
     (forall (i: nat). mask i /\ i < Seq.length v ==> Seq.index v i == Seq.index v' i))
   ensures pts_to_mask arr #f v' mask'
 
-fn mask_alloc #elt (x: elt) (n: SZ.t)
+fn mask_alloc u#a (#elt: Type u#a) {| small_type u#a |} (x: elt) (n: SZ.t)
   returns a: array elt
   ensures pts_to_mask a (Seq.create (SZ.v n) x) (fun _ -> True)
   ensures pure (length a == SZ.v n /\ is_full_array a)
 
-fn mask_free #elt (a: array elt) (#s: Ghost.erased (Seq.seq elt)) #mask
+fn mask_free u#a (#elt: Type u#a) (a: array elt) (#s: Ghost.erased (Seq.seq elt)) #mask
   requires pts_to_mask a s mask
   requires pure (forall i. mask i)
   requires pure (is_full_array a)
 
 ghost
-fn mask_share #a (arr:array a) (#s: Seq.seq a) #p #mask
+fn mask_share u#a (#a: Type u#a) (arr:array a) (#s: Seq.seq a) #p #mask
   requires pts_to_mask arr #p s mask
   ensures pts_to_mask arr #(p /. 2.0R) s mask
   ensures pts_to_mask arr #(p /. 2.0R) s mask
 
 [@@allow_ambiguous]
-ghost fn mask_gather #t (arr: array t) #p1 #p2 #s1 #s2 #mask1 #mask2
+ghost fn mask_gather u#a (#t: Type u#a) (arr: array t) #p1 #p2 #s1 #s2 #mask1 #mask2
   requires pts_to_mask arr #p1 s1 mask1
   requires pts_to_mask arr #p2 s2 mask2
   requires pure (forall i. mask1 i <==> mask2 i)
@@ -111,13 +112,13 @@ ghost fn mask_gather #t (arr: array t) #p1 #p2 #s1 #s2 #mask1 #mask2
 unfold let mask_isect (mask pred: nat -> prop) : nat -> prop = fun i -> mask i /\ pred i
 unfold let mask_diff (mask pred: nat -> prop) : nat -> prop = fun i -> mask i /\ ~(pred i)
 
-ghost fn split_mask #t (arr: array t) #f #v #mask (pred: nat -> prop)
+ghost fn split_mask u#a (#t: Type u#a) (arr: array t) #f #v #mask (pred: nat -> prop)
   requires pts_to_mask arr #f v mask
   ensures pts_to_mask arr #f v (mask_isect mask pred)
   ensures pts_to_mask arr #f v (mask_diff mask pred)
 
 [@@allow_ambiguous]
-ghost fn join_mask #t (arr: array t) #f #v1 #v2 #mask1 #mask2
+ghost fn join_mask u#a (#t: Type u#a) (arr: array t) #f #v1 #v2 #mask1 #mask2
   requires pts_to_mask arr #f v1 mask1
   requires pts_to_mask arr #f v2 mask2
   requires pure (forall i. ~(mask1 i /\ mask2 i))
@@ -129,7 +130,7 @@ ghost fn join_mask #t (arr: array t) #f #v1 #v2 #mask1 #mask2
         (mask2 i ==> Seq.index v i == Seq.index v2 i)))
 
 [@@allow_ambiguous]
-ghost fn join_mask' #t (arr: array t) #f (#v: erased (Seq.seq t)) #mask1 #mask2
+ghost fn join_mask' u#a (#t: Type u#a) (arr: array t) #f (#v: erased (Seq.seq t)) #mask1 #mask2
   requires pts_to_mask arr #f v mask1
   requires pts_to_mask arr #f v mask2
   requires pure (forall i. ~(mask1 i /\ mask2 i))
@@ -137,20 +138,20 @@ ghost fn join_mask' #t (arr: array t) #f (#v: erased (Seq.seq t)) #mask1 #mask2
 
 [@@allow_ambiguous]
 ghost
-fn pts_to_mask_injective_eq #a #p0 #p1 #s0 #s1 #mask0 #mask1 (arr:array a)
+fn pts_to_mask_injective_eq u#a (#a: Type u#a) #p0 #p1 #s0 #s1 #mask0 #mask1 (arr:array a)
   preserves pts_to_mask arr #p0 s0 mask0
   preserves pts_to_mask arr #p1 s1 mask1
   ensures pure (Seq.length s0 == Seq.length s1 /\
     (forall (i: nat). i < Seq.length s0 /\ mask0 i /\ mask1 i ==>
       Seq.index s0 i == Seq.index s1 i))
 
-fn mask_read #t (a: array t) (i: SZ.t) #p (#s: erased (Seq.seq t) { SZ.v i < Seq.length s }) #mask
+fn mask_read u#a (#t: Type u#a) (a: array t) (i: SZ.t) #p (#s: erased (Seq.seq t) { SZ.v i < Seq.length s }) #mask
   preserves pts_to_mask a #p s mask
   requires pure (mask (SZ.v i))
   returns res: t
   ensures pure (res == Seq.index s (SZ.v i))
 
-fn mask_write #t (a: array t) (i: SZ.t) (v: t) (#s: erased (Seq.seq t) { SZ.v i < Seq.length s }) #mask
+fn mask_write u#a (#t: Type u#a) (a: array t) (i: SZ.t) (v: t) (#s: erased (Seq.seq t) { SZ.v i < Seq.length s }) #mask
   requires pts_to_mask a s mask
   requires pure (mask (SZ.v i))
   ensures pts_to_mask a (Seq.upd s (SZ.v i) v) mask
@@ -161,13 +162,13 @@ val length_gsub #t arr i j : Lemma (length (gsub #t arr i j) == j - i) [SMTPat (
 val offset_of_gsub #t arr i j : Lemma (offset_of (gsub #t arr i j) == offset_of arr + i) [SMTPat (offset_of (gsub arr i j))]
 val base_of_gsub #t arr i j : Lemma (base_of (gsub #t arr i j) == base_of arr) [SMTPat (base_of (gsub arr i j))]
 
-ghost fn gsub_intro #t (arr: array t) #f #mask (i j: nat) (#v: erased (Seq.seq t) { i <= j /\ j <= Seq.length v })
+ghost fn gsub_intro u#a (#t: Type u#a) (arr: array t) #f #mask (i j: nat) (#v: erased (Seq.seq t) { i <= j /\ j <= Seq.length v })
   requires pts_to_mask arr #f v mask
   requires pure (forall (k: nat). mask k /\ k < Seq.length v ==> i <= k /\ k < j)
   returns _: squash (length arr == Seq.length v)
   ensures pts_to_mask (gsub arr i j) #f (Seq.slice v i j) (fun k -> mask (k + i))
 
-ghost fn gsub_elim #t (arr: array t) #f (#mask: nat->prop) (i j: nat)
+ghost fn gsub_elim u#a (#t: Type u#a) (arr: array t) #f (#mask: nat->prop) (i j: nat)
     (#v: erased (Seq.seq t) { i <= j /\ j <= length arr })
   requires pts_to_mask (gsub arr i j) #f v mask
   returns _: squash (j - i == Seq.length v)
@@ -176,7 +177,7 @@ ghost fn gsub_elim #t (arr: array t) #f (#mask: nat->prop) (i j: nat)
     pure (Seq.length v' == length arr /\ (forall (k:nat). k < j - i ==> Seq.index v k == Seq.index v' (k + i)))
 
 unobservable
-fn sub #t (arr: array t) #f #mask (i: SZ.t) (j: SZ.t)
+fn sub u#a (#t: Type u#a) (arr: array t) #f #mask (i: SZ.t) (j: SZ.t)
     (#v: erased (Seq.seq t) { SZ.v i <= SZ.v j /\ SZ.v j <= Seq.length (reveal v) })
   requires pts_to_mask arr #f v mask
   returns sub: (sub: array t { length arr == Seq.length (reveal v) })
@@ -185,7 +186,7 @@ fn sub #t (arr: array t) #f #mask (i: SZ.t) (j: SZ.t)
   ensures pts_to_mask arr #f v (fun k -> mask k /\ ~(SZ.v i <= k /\ k < SZ.v j))
 
 [@@allow_ambiguous]
-ghost fn return_sub #t (arr: array t) #f (#v #vsub: erased (Seq.seq t)) #mask #masksub (#i: nat) (#j: nat { i <= j /\ j <= length arr })
+ghost fn return_sub u#a (#t: Type u#a) (arr: array t) #f (#v #vsub: erased (Seq.seq t)) #mask #masksub (#i: nat) (#j: nat { i <= j /\ j <= length arr })
   requires pts_to_mask arr #f v mask
   requires pts_to_mask (gsub arr i j) #f vsub masksub
   requires pure (forall (k: nat). i <= k /\ k < j ==> ~(mask k))
