pulse/lib/pulse/lib/Pulse.Lib.SmallType.fst
@@ -1,0 +1,30 @@
+(*
+   Copyright 2025 Microsoft Research
+
+   Licensed under the Apache License, Version 2.0 (the "License");
+   you may not use this file except in compliance with the License.
+   You may obtain a copy of the License at
+
+       http://www.apache.org/licenses/LICENSE-2.0
+
+   Unless required by applicable law or agreed to in writing, software
+   distributed under the License is distributed on an "AS IS" BASIS,
+   WITHOUT WARRANTIES OR CONDITIONS OF ANY KIND, either express or implied.
+   See the License for the specific language governing permissions and
+   limitations under the License.
+*)
+module Pulse.Lib.SmallType
+module U = Pulse.Lib.Raise
+
+// Type class of types that can be stored in a reference
+[@@Tactics.Typeclasses.tcclass; erasable]
+let small_type = U.raisable u#a u#2
+
+instance small_type_non_info : Pulse.Lib.NonInformative.non_informative (small_type u#a) =
+  U.raisable_non_info
+
+instance small_type0 : small_type u#0 = U.raisable_inst
+instance small_type1 : small_type u#1 = U.raisable_inst u#1 u#2
+instance small_type2 : small_type u#2 = U.raisable_inst u#2 u#2
+
+instance of_small_type {| inst : small_type u#a |} : U.raisable u#a u#2 = inst
